Complete mergesort example

WfInduct/MergeSort.lean
@@ -1,7 +1,7 @@
 import WfInduct.Basic
 import Std
 
-def merge (r : α → α → Bool) : (l : List α) → (l' : List α) → List α
+def merge (r : α → α → Prop) [DecidableRel r] : (l : List α) → (l' : List α) → List α
   | [], l' => l'
   | l, [] => l
   | a :: l, b :: l' => if r a b then a :: merge r l (b :: l') else b :: merge r (a :: l) l'
@@ -10,17 +10,16 @@ def merge (r : α → α → Bool) : (l : List α) → (l' : List α) → List �
 derive_induction merge
 
 /--
-info: merge.induct.{u_1} {α : Type u_1} (r : α → α → Bool) (motive : List α → List α → Prop)
+info: merge.induct.{u_1} {α : Type u_1} (r : α → α → Prop) [inst✝ : DecidableRel r] (motive : List α → List α → Prop)
   (case1 : ∀ (l' : List α), motive [] l') (case2 : ∀ (l : List α), (l = [] → False) → motive l [])
-  (case3 : ∀ (a : α) (l : List α) (b : α) (l' : List α), r a b = true → motive l (b :: l') → motive (a :: l) (b :: l'))
-  (case4 : ∀ (a : α) (l : List α) (b : α) (l' : List α), ¬r a b = true → motive (a :: l) l' → motive (a :: l) (b :: l'))
+  (case3 : ∀ (a : α) (l : List α) (b : α) (l' : List α), r a b → motive l (b :: l') → motive (a :: l) (b :: l'))
+  (case4 : ∀ (a : α) (l : List α) (b : α) (l' : List α), ¬r a b → motive (a :: l) l' → motive (a :: l) (b :: l'))
   (x x : List α) : motive x x
 -/
 #guard_msgs in
 #check merge.induct
 
--- just a warmup
-theorem perm_length (l : List α) (l' : List α) :
+theorem merge_length (r : α → α → Prop) [DecidableRel r] (l : List α) (l' : List α) :
     (merge r l l').length = l.length + l'.length := by
   induction l, l' using merge.induct (r := r) -- NB: Needs lean4#3188
   case case1 => simp [merge]
@@ -32,3 +31,110 @@ theorem perm_length (l : List α) (l' : List α) :
   case case4 a l b l' hr IH =>
     simp only [merge, hr, ↓reduceIte]
     simp_arith [IH]
+
+open List in
+theorem merge_perm (r : α → α → Prop) [DecidableRel r] (l l' : List α) : merge r l l' ~ l ++ l' := by
+  induction l, l' using merge.induct (r := r)
+  case case1 l => simp [merge]
+  case case2 l overlap => simp [merge]
+  case case3 a l b l' hr IH => simpa [merge, hr] using IH
+  case case4 a l b l' hr IH =>
+    suffices b :: merge r (a :: l) l' ~ a :: (l ++ b :: l') by simpa [merge, hr]
+    exact (IH.cons _).trans ((Perm.swap _ _ _).trans (perm_middle.symm.cons _))
+
+theorem merge_pairwise (r : α → α → Prop) [DecidableRel r]
+    (trans : ∀ {a b c}, r a b → r b c → r a c)
+    (total : ∀ a b, r a b ∨ r b a )
+    {l l' : List α} (h₁ : l.Pairwise r) (h₂ : l'.Pairwise r) : (merge r l l').Pairwise r := by
+  induction l, l' using merge.induct (r := r)
+  case case1 l => simpa only [merge] using h₂
+  case case2 l hoverlap => simpa only [merge] using h₁
+  case case3 a l b l' hr IH =>
+    suffices ∀ b' ∈ merge r l (b :: l'), r a b' by
+      simpa [merge, hr, IH h₁.of_cons h₂]
+    intro b' bm
+    rcases show b' = b ∨ b' ∈ l ∨ b' ∈ l' by
+        simpa [or_left_comm] using (merge_perm _ _ _).subset bm with
+      (be | bl | bl')
+    · subst b'
+      assumption
+    · exact List.rel_of_pairwise_cons h₁ bl
+    · exact trans hr (List.rel_of_pairwise_cons h₂ bl')
+  case case4 a l b l' hr IH =>
+    suffices ∀ a' ∈ merge r (a :: l) l', r b a' by
+      simpa [merge, hr, IH h₁ h₂.of_cons]
+    replace hr : r b a := by cases total a b <;> [contradiction ; assumption]
+    intro a' am
+    rcases show a' = a ∨ a' ∈ l ∨ a' ∈ l' by
+        simpa [or_right_comm] using (merge_perm _ _ _).subset am with
+      (ae | al | al')
+    · subst a'
+      assumption
+    · exact trans hr (List.rel_of_pairwise_cons h₁ al)
+    · exact List.rel_of_pairwise_cons h₂ al'
+
+
+@[simp]
+def split (l : List α) : List α × List α :=
+  (l.take (l.length / 2), l.drop (l.length / 2))
+
+def mergeSort (r : α → α → Prop) [DecidableRel r] (l : List α) : List α :=
+  let n := l.length
+  if n < 2
+    then l
+  else
+    merge r (mergeSort r (l.take (n/2))) (mergeSort r (l.drop (n/2)))
+termination_by l.length
+decreasing_by
+ · simp_wf; simp only [Nat.min_def]; split <;> omega
+ · simp_wf; omega
+
+derive_induction mergeSort
+
+/--
+info: mergeSort.induct.{u_1} {α : Type u_1} (r : α → α → Prop) [inst✝ : DecidableRel r] (motive : List α → Prop)
+  (case1 :
+    ∀ (x : List α),
+      let n := List.length x;
+      n < 2 → motive x)
+  (case2 :
+    ∀ (x : List α),
+      let n := List.length x;
+      ¬n < 2 → motive (List.take (n / 2) x) → motive (List.drop (n / 2) x) → motive x)
+  (x : List α) : motive x
+-/
+#guard_msgs in
+#check mergeSort.induct
+
+theorem List.pairwise_of_length_lt_2 {r : α → α → Prop} :
+    ∀ {l : List α},  l.length < 2 → l.Pairwise r
+  | [], _ => List.Pairwise.nil
+  | [x], _ => by simp [List.Pairwise]
+  | (_::_::_), h => by contradiction
+
+theorem mergeSort_pairwise (r : α → α → Prop) [DecidableRel r]
+    (trans : ∀ {a b c}, r a b → r b c → r a c)
+    (total : ∀ a b, r a b ∨ r b a )
+    {l : List α} : (mergeSort r l).Pairwise r := by
+  induction l using  mergeSort.induct (r := r)
+  case case1 l n =>
+    intro h -- TODO: the induction tactic seems to miscount params, maybe due to the let
+    unfold mergeSort; simp [h]
+    exact List.pairwise_of_length_lt_2 h
+  case case2 l n h IH₁ =>
+    intro IH₂ -- TODO: the induction tactic seems to miscount params, maybe due to the let
+    unfold mergeSort; simp [h]
+    apply merge_pairwise r trans total IH₁ IH₂
+
+open List in
+theorem mergeSort_perm (r : α → α → Prop) [DecidableRel r] (l : List α) : mergeSort r l ~ l := by
+  induction l using mergeSort.induct (r := r)
+  case case1 l n =>
+    intro h
+    simp [mergeSort, h]
+  case case2 l n h IH₁ =>
+    intro IH₂
+    unfold mergeSort; simp [h] -- simp [mergeSort] does not work well here
+    apply (merge_perm _ _ _).trans
+    apply (Perm.append IH₁ IH₂).trans
+    simp only [take_append_drop, Perm.refl]
